Weakest precondition start, use mapping lookup, option to result function

Result.thy
@@ -26,8 +26,17 @@ definition return :: "'a \<Rightarrow> 'a result" where
 adhoc_overloading
   Monad_Syntax.bind==bind
 
-
 fun assert where "assert e True = ok ()" | "assert e False = err e"
+
+fun some_or_err :: "'a option \<Rightarrow> error \<Rightarrow> 'a result" where
+  "some_or_err (Some v) _ = ok v"
+| "some_or_err None e = err e"
+
+definition wp :: "'a result \<Rightarrow> ('a \<Rightarrow> bool) \<Rightarrow> (error \<Rightarrow> bool) \<Rightarrow> bool" where
+  "wp m P E = (case m of ok v \<Rightarrow> P v | err e \<Rightarrow> E e)"
+
+definition wp_ok :: "'a result \<Rightarrow> ('a \<Rightarrow> bool) \<Rightarrow> bool" where
+  "wp_ok m P = wp m P (\<lambda>x. True)"
 
 
 
@@ -81,6 +90,42 @@ lemma result_return_ok_iff[simp]: "return x = ok y \<longleftrightarrow> x = y"
   by simp
 
 end
+
+
+subsection "Weakest precondition simps"
+
+lemma wp_ok_iff[simp]: "wp (ok v) P E \<longleftrightarrow> (P v)"
+  unfolding wp_def
+  by simp
+
+lemma wp_ok_ok_iff[simp]: "wp_ok (ok v) P \<longleftrightarrow> (P v)"
+  unfolding wp_ok_def
+  by simp
+
+lemma wp_err_iff[simp]: "wp (err e) P E \<longleftrightarrow> (E e)"
+  unfolding wp_def
+  by simp
+
+lemma wp_ok_err_iff[simp]: "wp_ok (err e) P \<longleftrightarrow> True"
+  unfolding wp_ok_def
+  by simp
+
+lemma wp_return_iff[simp]: "wp (return x) P E \<longleftrightarrow> (P x)"
+  unfolding return_def wp_def
+  by simp
+
+lemma wp_ok_return_iff[simp]: "wp_ok (return x) P \<longleftrightarrow> (P x)"
+  unfolding wp_ok_def
+  by simp
+
+lemma wp_bind_iff[simp]: "wp (do {x \<leftarrow> m; f x}) P E \<longleftrightarrow> ((\<exists>x. m = ok x \<and> (wp (f x) P E)) \<or> (\<exists>e. m = err e \<and> E e))"
+  unfolding wp_def bind_def
+  by (cases m; simp)
+
+lemma wp_ok_bind_iff[simp]: "wp_ok (do {x \<leftarrow> m; f x}) P \<longleftrightarrow> ((\<exists>x. m = ok x \<and> (wp_ok (f x) P)) \<or> (\<exists>e. m = err e))"
+  unfolding wp_ok_def
+  by simp
+
 
 (* TODO: MONADIC IF *)
 
